mppa_k1c/Asmblockgenproof1.v
@@ -1277,16 +1277,16 @@ Proof.
 *)*)
 Qed.
 
-(*
+
 Lemma indexed_load_access_correct:
-  forall chunk (mk_instr: ireg -> offset -> instruction) rd m,
+  forall chunk (mk_instr: ireg -> offset -> basic) rd m,
   (forall base ofs rs,
-     exec_instr ge fn (mk_instr base ofs) rs m = exec_load ge chunk rs m rd base ofs) ->
+     exec_basic_instr ge (mk_instr base ofs) rs m = exec_load ge chunk rs m rd base ofs) ->
   forall (base: ireg) ofs k (rs: regset) v,
   Mem.loadv chunk m (Val.offset_ptr rs#base ofs) = Some v ->
   base <> GPR31 -> rd <> PC ->
   exists rs',
-     exec_straight ge fn (indexed_memory_access mk_instr base ofs k) rs m k rs' m
+     exec_straight ge (indexed_memory_access mk_instr base ofs :: k) rs m k rs' m
   /\ rs'#rd = v
   /\ forall r, r <> PC -> r <> GPR31 -> r <> rd -> rs'#r = rs#r.
 Proof.
@@ -1296,11 +1296,8 @@ Proof.
   econstructor; split.
   eapply exec_straight_opt_right. eexact A. apply exec_straight_one. rewrite EXEC.
   unfold exec_load. rewrite B, LOAD. eauto. Simpl. 
-  split; intros; Simpl.
+  split; intros; Simpl. auto.
 Qed.
-*)
-
-Definition noscroll := 0.
 
 Lemma indexed_store_access_correct:
   forall chunk (mk_instr: ireg -> offset -> basic) r1 m,
@@ -1308,7 +1305,7 @@ Lemma indexed_store_access_correct:
      exec_basic_instr ge (mk_instr base ofs) rs m = exec_store ge chunk rs m r1 base ofs) ->
   forall (base: ireg) ofs k (rs: regset) m',
   Mem.storev chunk m (Val.offset_ptr rs#base ofs) (rs#r1) = Some m' ->
-  base <> GPR31 -> r1 <> GPR31 -> IR r1 <> PC ->
+  base <> GPR31 -> r1 <> GPR31 -> r1 <> PC ->
   exists rs',
      exec_straight ge (indexed_memory_access mk_instr base ofs :: k) rs m k rs' m'
   /\ forall r, r <> PC -> r <> GPR31 -> rs'#r = rs#r.
@@ -1318,12 +1315,9 @@ Proof.
   intros (base' & ofs' & rs' & A & B & C).
   econstructor; split.
   eapply exec_straight_opt_right. eapply A. apply exec_straight_one. rewrite EXEC.
-  unfold exec_store. rewrite B, C, STORE. eauto. eauto. 
-  destruct r1; try discriminate. contradiction NOT31'. auto. auto.
-(*   intros; Simpl. *)
+  unfold exec_store. rewrite B, C, STORE. eauto. eauto. auto.
+  intros; Simpl. rewrite C; auto.
 Qed.
-
-
 
 Lemma loadind_correct:
   forall (base: ireg) ofs ty dst k c (rs: regset) m v,
@@ -1334,41 +1328,38 @@ Lemma loadind_correct:
      exec_straight ge c rs m k rs' m
   /\ rs'#(preg_of dst) = v
   /\ forall r, r <> PC -> r <> GPR31 -> r <> preg_of dst -> rs'#r = rs#r.
-Proof. Admitted.
-(*   intros until v; intros TR LOAD NOT31. 
+Proof.
+  intros until v; intros TR LOAD NOT31. 
   assert (A: exists mk_instr,
-                c = indexed_memory_access mk_instr base ofs k
+                c = indexed_memory_access mk_instr base ofs :: k
              /\ forall base' ofs' rs',
-                   exec_instr ge fn (mk_instr base' ofs') rs' m =
+                   exec_basic_instr ge (mk_instr base' ofs') rs' m =
                    exec_load ge (chunk_of_type ty) rs' m (preg_of dst) base' ofs').
   { unfold loadind in TR.
     destruct ty, (preg_of dst); inv TR; econstructor; split; eauto. }
   destruct A as (mk_instr & B & C). subst c. 
   eapply indexed_load_access_correct; eauto with asmgen. 
-Qed. *)
+Qed.
 
-(*
 Lemma storeind_correct:
   forall (base: ireg) ofs ty src k c (rs: regset) m m',
   storeind src base ofs ty k = OK c ->
   Mem.storev (chunk_of_type ty) m (Val.offset_ptr rs#base ofs) rs#(preg_of src) = Some m' ->
   base <> GPR31 ->
   exists rs',
-     exec_straight ge fn c rs m k rs' m'
+     exec_straight ge c rs m k rs' m'
   /\ forall r, r <> PC -> r <> GPR31 -> rs'#r = rs#r.
 Proof.
-  intros until m'; intros TR STORE NOT31. 
+  intros until m'; intros TR STORE NOT31.
   assert (A: exists mk_instr,
-                c = indexed_memory_access mk_instr base ofs k
+                c = indexed_memory_access mk_instr base ofs :: k
              /\ forall base' ofs' rs',
-                   exec_instr ge fn (mk_instr base' ofs') rs' m =
+                   exec_basic_instr ge (mk_instr base' ofs') rs' m =
                    exec_store ge (chunk_of_type ty) rs' m (preg_of src) base' ofs').
   { unfold storeind in TR. destruct ty, (preg_of src); inv TR; econstructor; split; eauto. }
   destruct A as (mk_instr & B & C). subst c. 
   eapply indexed_store_access_correct; eauto with asmgen. 
 Qed.
-
-*)
 
 Ltac bsimpl := unfold exec_bblock; simpl.
 
